sf/Assignment08_11.v
@@ -2,12 +2,34 @@ Require Export Assignment08_10.
 
 (* problem #11: 10 points *)
 
+Definition beq_id (X1 : id) (X2 : id) : bool :=
+  match (X1, X2) with
+    (Id x1, Id x2) => beq_nat x1 x2
+  end.
+
+Theorem update_same : forall n1 x1 x2 (st : state),
+  st x1 = n1 ->
+  (update st x1 n1) x2 = st x2.
+Proof.
+  intros. unfold update. remember (beq_id x1 x2). destruct b.
+  - destruct (eq_id_dec x1 x2). subst. reflexivity. reflexivity.
+  - destruct (eq_id_dec x1 x2). subst. reflexivity. reflexivity.
+Qed.
+
 (** **** Exercise: 2 stars (assign_aequiv)  *)
 Theorem assign_aequiv : forall X e,
   aequiv (AId X) e -> 
   cequiv SKIP (X ::= e).
 Proof.
-  exact FILL_IN_HERE.
+  intros. split ; intros.
+  - inversion H0 ; subst. assert ((update st' X (aeval st' e)) = st').
+    + unfold aequiv in H. rewrite <- H. simpl. apply functional_extensionality. intros. 
+      apply update_same. reflexivity.
+    + rewrite <- H1 at 2. apply E_Ass. reflexivity.
+  - inversion H0 ; subst. assert ((update st X (aeval st e)) = st).
+    + unfold aequiv in H. simpl in H. rewrite <- H. apply functional_extensionality. intros. 
+      apply update_same. reflexivity.
+    + rewrite H1. apply E_Skip.
 Qed.
 
 (*-- Check --*)
