sf/Assignment08_02.v
@@ -12,7 +12,7 @@ Definition pup_to_n : com :=
   Y ::= ANum 0;;
   WHILE BNot (BEq (AId X) (ANum 0)) DO
     Y ::= APlus (AId Y) (AId X);;
-    Z ::= AMinus (AId X) (ANum 1)
+    X ::= AMinus (AId X) (ANum 1)
   END.
 
 Example pup_to_2_ceval :
@@ -21,14 +21,16 @@ Example pup_to_2_ceval :
       X 2) Y 0) Y 2) X 1) Y 3) X 0.
 Proof.
   unfold pup_to_n. apply E_Seq with (st':= update (update empty_state X 2) Y 0).
-  - apply E_Ass. simpl. reflexivity.
-  - apply E_WhileLoop with (st' := (update (update (update (update empty_state X 2) Y 0) Y 2) X 1)).
-    + simpl.
-  
-
-  unfold pup_to_n. 
-  - 
-
+  apply E_Ass. simpl. reflexivity.
+  apply E_WhileLoop with (st' := (update (update (update (update empty_state X 2) Y 0) Y 2) X 1)).
+  - simpl. reflexivity.
+  - apply E_Seq with (st' := (update (update (update empty_state X 2) Y 0) Y 2)); try (apply E_Ass; simpl; reflexivity).
+  - apply E_WhileLoop with (st' := (update (update (update (update (update (update empty_state X 2) Y 0) Y 2) X 1)
+                              Y 3) X 0)).
+    + simpl. reflexivity.
+    + apply E_Seq with (st' := (update (update (update (update (update empty_state X 2) Y 0) Y 2) X 1) Y 3)) ;
+      try (apply E_Ass; compute; reflexivity).
+    + apply E_WhileEnd. simpl. reflexivity.
 Qed.
 
 (*-- Check --*)
