sf/Assignment08_10.v
@@ -6,7 +6,12 @@ Require Export Assignment08_09.
 Theorem seq_assoc : forall c1 c2 c3,
   cequiv ((c1;;c2);;c3) (c1;;(c2;;c3)).
 Proof.
-  exact FILL_IN_HERE.
+  split ; intros.
+  - inversion H ; subst. inversion H2 ; subst.
+    apply E_Seq with (st' := st'1). assumption.
+    apply E_Seq with (st' := st'0) ; assumption. 
+  - inversion H ; subst. inversion H5 ; subst.
+    apply E_Seq with (st' := st'1). apply E_Seq with (st' := st'0) ; assumption. assumption.
 Qed.
 
 (*-- Check --*)
